verify push_back

examples.v
@@ -4,30 +4,16 @@ Require Export lang.
 From iris.bi Require Import bi.
 Require Export ISL.
 
-(* in this example v is a (EVal (VLoc n))
-   describing in the location in the heap where
-   we will find a second location. In C parlance
-   this would be a
-   v ** int so a pointer to a vector of integers.
 
-   In our case the underlying vector is just one cell
-   so we can free and allocate just one to simulate
-   a use after free bug later on.
- *)
-
- Definition push_back : expr → expr := λ v,
+Definition push_back : expr → expr := λ v,
     (ELet "z" EAmb
           (EIf (EOp EqOp (EVar "z") (EVal (VNat 0)))
                (EVal VUnit)
-               (ELet "y" (ELoad v) (* now y points to the underlying array *)
-                     (ESeq (EFree (EVar "y"))
-                           (ELet "y" (EAlloc (EVal (VNat 42)))
-                                 (EStore v (EVar "y"))))))).
+               (ELet "old" (ELoad v) (* now y points to the underlying array *)
+                     (ELet "new" (EAlloc (ELoad (EVar "old"))) (* copy the value *)
+                           (ESeq (EFree (EVar "old"))
+                                 (EStore v (EVar "new"))))))).
 
-Example example_push_back := push_back (EVal (VLoc 0)).
-Check example_push_back.
-Print example_push_back.
-Compute example_push_back.
 
 (* client is where we will trigger the use-after-free
    error as we get a hold of a location that might be
@@ -41,237 +27,83 @@ Definition client : expr :=
           (ESeq (push_back (EVar "v")) (* here the underlying storage for v might be moved *)
                 (EStore (EVar "x") (EVal (VNat 88))))))). (* so using the previous location might fault *)
 
-(*
-Lemma client_can_error : will_error iEmpty client.
+Lemma push_back_ok v a b: hoare (v ↦ (VLoc a) ∗ a ↦ b)%S (push_back (EVal (VLoc v))) (λ r, ∃ a', @[ r = VUnit ] ∗ v ↦ (VLoc a') ∗ a' ↦ b ∗ a ↦ ⊥ )%S.
 Proof.
-  unfold will_error, client.
-  exists empty.
-  (* {[ 0 := (VNat 0) ]} ∪ {[ 1 := (VLoc 0) ]} ∪ {[ 2 := (VNat 42) ]}. *)
-  exists ({[ 0 := Reserved ]} ∪ {[ 1 := (Value (VLoc 2)) ]} ∪ {[ 2 := (Value (VNat 42)) ]}).
-  exists (EStore (EVal (VLoc 0)) (EVal (VNat 88))).
-  split; [done |].
-  split.
-  - eapply steps_trans.
-    eapply steps_let_val'.
-    + apply steps_single.
-      apply (Alloc_headstep ∅ (VNat 0) 0).
-      unfold valid_alloc.
-      intros e H.
-      exfalso.
-      eapply lookup_empty_is_Some.
-      eexists e.
-      eauto.
-    + rewrite insert_empty.
-      simpl subst.
-      eapply steps_trans.
-      eapply steps_let_val'.
-      * apply steps_single.
-        apply (Alloc_headstep {[0:= (Value (VNat 0))]} (VLoc 0) 1).
-        unfold valid_alloc.
-        rewrite lookup_singleton_ne.
-        discriminate.
-        auto.
-      * simpl subst.
-        rewrite insert_union_singleton_l.
-        eapply steps_trans.
-        eapply steps_let_val'.
-        -- apply steps_single.
-           econstructor.
-           eapply lookup_union_Some; auto.
-           rewrite map_disjoint_singleton_l. auto using lookup_singleton_None.
-        -- simpl subst.
-           eapply steps_seq_val'.
-           ++ eapply steps_trans.
-              eapply steps_let_val'.
-              ** apply steps_single.
-                 apply (Amb_headstep ({[1 := (Value (VLoc 0))]} ∪ {[0 := (Value (VNat 0))]}) 1).
-              ** simpl subst.
-                 eapply steps_trans.
-                 apply steps_if_false'.
-                 --- eauto using steps_single, head_step.
-                 --- eapply steps_trans. apply steps_let_val'.
-                     +++ eauto using steps_single, head_step.
-                     +++ simpl subst.
-                         eapply steps_seq_val'.
-                         *** eauto using steps_single, head_step.
-                         *** eapply steps_trans.
-                             ---- apply steps_let_val'.
-                                  apply steps_single.
-                                  rewrite insert_union_r.
-                                  rewrite insert_singleton.
-                                  apply (Alloc_headstep ({[1 := Value (VLoc 0)]} ∪ {[0 := Reserved]}) (VNat 42) 2).
-                                  unfold valid_alloc.
-                                  intros.
-                                  erewrite lookup_union_Some in H.
-                                  destruct H as [H | H]; rewrite lookup_singleton_ne in H; discriminate.
-                                  solve_map_disjoint.
-                                  auto using lookup_singleton_ne.
-                             ---- simpl subst.
-                                  apply steps_single.
-                                  eauto using head_step.
-           ++ rewrite insert_commute; eauto.
-              rewrite insert_union_l.
-              rewrite insert_union_singleton_r.
-              rewrite insert_singleton.
-              assert (
-                  ({[1 := Value (VLoc 2)]} ∪ {[0 := Reserved]} : mem)
-                  =
-                  ({[0 := Reserved]} ∪ {[1 := Value (VLoc 2)]})
-              ).
-              { admit. }
-              assert (
-                  ({[1 := Value (VLoc 2)]} ∪ {[0 := Reserved]} ∪ {[2 := Value (VNat 42)]}: mem)
-                  =
-                  ({[0 := Reserved]} ∪ {[1 := Value (VLoc 2)]} ∪ {[2 := Value (VNat 42)]})
-              ).
-              { admit. }
-              rewrite H0.
-              apply steps_refl.
-              rewrite lookup_union_None.
-              split; simpl_map; reflexivity.
-  - unfold is_error.
-    split.
-    + auto.
-    + intros.
-      intro.
-      erewrite step_store_inv in H. destruct H as (w & lookup_h & _ & _).
-      do 2 erewrite lookup_union_Some in lookup_h.
-      destruct lookup_h as [ [a|b] | c].
-      * rewrite lookup_singleton in a.
-        discriminate.
-      * rewrite lookup_singleton_ne in b.
-        discriminate.
-        auto.
-      * rewrite lookup_singleton_ne in c.
-        discriminate.
-        auto.
-      * solve_map_disjoint.
-      * solve_map_disjoint.
-      * solve_map_disjoint.
-Admitted.
-
-
-(* now this example may error if the test evaluates to true *)
-Example may_error := (EIf amb_bool EError (EVal VUnit)).
-
-Lemma may_error_contains_error : ∀ m,  contains_error may_error m.
-Proof.
-  unfold contains_error, may_error, amb_bool.
-  intros.
-  eexists EError, m.
-  split.
-  - apply (steps_step
-             m m m
-             (EIf (EOp EqOp EAmb (EVal (VNat 0))) EError (EVal VUnit))
-             (EIf (EOp EqOp (EVal (VNat 0)) (EVal (VNat 0))) EError (EVal VUnit))).
-    + change (EIf (EOp EqOp EAmb (EVal (VNat 0))) EError (EVal VUnit)) with
-          (fill [(IfCtx EError (EVal VUnit)); (OpCtxL EqOp (EVal (VNat 0)))] EAmb).
-      change (EIf (EOp EqOp (EVal (VNat 0)) (EVal (VNat 0))) EError (EVal VUnit)) with
-          (fill [(IfCtx EError (EVal VUnit)); (OpCtxL EqOp (EVal (VNat 0)))] (EVal (VNat 0))).
-      constructor.
-      constructor.
-    + apply (steps_step
-             m m m
-             (EIf (EOp EqOp (EVal (VNat 0)) (EVal (VNat 0))) EError (EVal VUnit))
-             (EIf (EVal (VBool true)) EError (EVal VUnit))).
-      * change (EIf (EOp EqOp (EVal (VNat 0)) (EVal (VNat 0))) EError (EVal VUnit)) with
-            (fill [(IfCtx EError (EVal VUnit))] (EOp EqOp (EVal (VNat 0)) (EVal (VNat 0)))).
-        change (EIf (EVal (VBool true)) EError (EVal VUnit)) with
-            (fill [(IfCtx EError (EVal VUnit))] (EVal (VBool true))).
-        constructor.
-        constructor.
+  apply hoare_exists_forallS; intros.
+  unfold push_back.
+  eapply hoare_let.
+  - eapply hoare_consS.
+    + apply iSep_emp_l_inv.
+    + intros. apply iEntails_refl.
+    + simpl.
+      apply (hoare_frame_r (v ↦ VLoc a ∗ a ↦ b) emp (λ v1 : val, @[ v1 = (VNat 1) ]))%S.
+      apply hoare_amb.
+  - simpl.
+    eapply hoare_if_false.
+    + eapply hoare_consS.
+      * apply iSep_emp_l_inv.
+      * intros. apply iEntails_refl.
+      * simpl.
+        apply (hoare_frame_r (v ↦ VLoc a ∗ a ↦ b) emp (λ v1 : val, (@[ v1 = VBool false])))%S.
+        apply hoare_op.
         simpl.
         reflexivity.
-      * apply steps_if_true.
-  - unfold is_error.
-    split; auto.
-    intros.
-    intro.
-    inversion H.
-    destruct E; simpl in *.
-    + subst.
-      inversion H1.
-    + destruct c; simpl in *; discriminate || auto.
+    + simpl.
+      eapply (hoare_let (λ r: val, v ↦ VLoc a ∗ a ↦ b))%S.
+      * eapply (hoare_consS (v ↦ (VLoc a) ∗a ↦ b)
+                            (λ r, @[r = (VLoc a)] ∗ v ↦ (VLoc a) ∗ (a ↦ b)))%S.
+        -- eapply iEntails_trans.
+           ++ apply iSep_comm.
+           ++ apply iSep_comm.
+        -- intros. apply iEntails_refl.
+        -- eapply hoare_consS.
+           ++ apply iEntails_refl.
+           ++ intro. apply iSep_assoc.
+           ++ simpl. apply hoare_frame_r. apply hoare_loadS.
+      * simpl.
+        apply (hoare_let (λ r : val, x ↦ b ∗ a ↦ b ∗ v ↦ (VLoc a)) (VLoc x))%S.
+        -- eapply hoare_consS.
+           ++ apply iSep_comm.
+           ++ intro.
+              ** eapply iEntails_trans.
+                 --- apply iSep_assoc.
+                 --- apply iSep_assoc.
+           ++ simpl.
+              eapply hoare_frame_r.
+              eapply (hoare_ctxS' [(AllocCtx)])%S.
+              apply (hoare_loadS a b).
+              simpl.
+              eapply hoare_consS.
+              ** apply iSep_emp_l_inv.
+              ** intro.
+                 apply iEntails_refl.
+              ** simpl. apply hoare_frame_r.
+                 apply hoare_alloc.
+        -- simpl.
+           eapply (hoare_seqS (λ r: val, a ↦ ⊥ ∗ x ↦ b ∗ v ↦ VLoc a) VUnit)%S.
+           ++ eapply (hoare_consS ((a ↦ b ) ∗ x ↦ b ∗ v ↦ VLoc a)
+                                  (λ r: val, (λ r : val, @[r=VUnit] ∗ a ↦ ⊥) r ∗ (x ↦ b ∗ v ↦ VLoc a)))%S.
+              ** eapply iEntails_trans.
+                 --- apply iSep_assoc.
+                 --- eapply iEntails_trans.
+                     +++ apply iSep_mono_l. apply iSep_comm.
+                     +++ apply iSep_assoc'.
+              ** intro. apply iSep_assoc.
+              ** eapply hoare_frame_r.
+                 apply hoare_freeS.
+           ++ eapply hoare_consS.
+              ** apply iSep_comm.
+              ** intro. eapply iEntails_trans. apply iSep_assoc. apply iSep_assoc.
+              ** simpl. apply hoare_frame_r.
+                 eapply hoare_consS.
+                 --- apply iSep_comm.
+                 --- intro. apply iEntails_refl.
+                 --- simpl.
+                     apply hoare_frame_r.
+                     apply hoare_storeS.
 Qed.
 
-(* finally we can now start messing around with our definitions
-   and prove that some expressions will error *)
 
-   Example simple_error := is_error EError ∅.
-
-   Lemma our_first_error : simple_error.
-   Proof.
-     unfold simple_error.
-     split.
-     - auto.
-     - intros.
-       unfold not.
-       intro.
-       (* now we got a proof of head_step for an expression EError
-          which is not a thing in our operational semantic; the contradiction
-          must come from there.
-        *)
-       inversion H.
-       (* the inversion left us with an _unknown_ context E to work with
-          but we still have the restriction that fill E e1 = EError; this
-          only makes sense when E = [] and e1 = EError *)
-       destruct E.
-       * simpl in *; subst; inversion H1.
-       * destruct c; simpl in *; discriminate.
-   Qed.
-
-   (* and we can get errors also from using resources wrongly *)
-
-   Lemma resource_error l: is_error (EFree (EVal (VLoc l))) ∅.
-   Proof.
-     split; [auto|].
-     intros ???H.
-     erewrite step_free_inv in H.
-     destruct H as (v & _ & lookup & _).
-     rewrite lookup_empty in lookup.
-     discriminate.
-   Qed.
-
-   Definition amb_bool := (EOp EqOp EAmb (EVal (VNat 0))).
-
-(* and finally prove that we can always get any two booleans *)
-Lemma amb_is_ambiguous (b : bool) (m : mem) : steps amb_bool m (EVal (VBool b)) m.
-Proof.
-  unfold amb_bool.
-  eapply steps_step.
-  rewrite <- fill_op_l.
-  constructor.
-  apply (Amb_headstep m (if b then 0 else 1)).
-  rewrite fill_op_l.
-  apply steps_single.
-  destruct b; eauto using head_step.
-Qed.
- *)
-
-(* Finally we can prove the same incorrectness specifications using the fancier rules *)
-Lemma simple_error':
-  hoare_err iEmp EError iEmp.
-Proof.
-  apply hoare_error.
-Qed.
-
-Lemma double_free l:
-  hoare_err (iNegPoints l) (EFree (EVal (VLoc l))) (iNegPoints l).
-Proof.
-  apply hoare_freeN.
-Qed.
-
-Lemma double_free' l v:
-  hoare_err (iPoints l v) (ESeq (EFree (EVal (VLoc l))) (EFree (EVal (VLoc l)))) (iNegPoints l).
-Proof.
-  eapply hoare_seqSN.
-  eapply hoare_freeS.
-  apply hoare_freeN.
-Qed.
-
-Lemma push_back_ok v a: hoare (∃ b,  v ↦ (VLoc a) ∗ a ↦ b)%S (push_back (EVal (VLoc v))) (λ r, ⌜ r = VUnit ⌝ ∗ ∃ a' b, v ↦ (VLoc a') ∗ a' ↦ b ∗ a ↦ ⊥ )%S.
-Proof.
-Admitted.
 
 Lemma client_error: hoare_err iEmp client ( 0 ↦ ⊥ ∗ 1 ↦ (VLoc 2) ∗ 2 ↦ VNat 42)%S.
 Proof.
